loop invariants for serialize_length, major steps for loop correctness [skip ci]

src/Lib/DWT/ExecBer_tlv_length_serialize.v
@@ -3,8 +3,6 @@ Require Import Core.Core Core.Notations.
 
 Open Scope IntScope.
 
-
-
 Program Fixpoint required_size_loop v i l {measure (Z.to_nat (Int.unsigned (Int.repr 32 - i)))}:=
   if (i <u Int.repr 32) 
   then if (v >> i) == 0
@@ -22,29 +20,18 @@ Fixpoint serialize_length_loop i n l :=
   | S n => (l >> i) :: serialize_length_loop (i - Int.repr 8) n l 
   end. 
 
-(* Definition serialize_length l := 
-  let n := Z.to_nat (Int.unsigned (required_size l)) 
-  serialize_length_loop n *)
-  
-Fixpoint serialize_tag_loop  n i tval :=
-  match n with
-  | O => []
-  | S n => (Int.repr 128 or (tval >> i & Int.repr 127)) 
-            :: serialize_tag_loop n (i - Int.repr 7) tval
-  end. 
-
-Definition serialize_tag' tval :=
-  let s := byte_length' tval in 
-  let n := Z.to_nat (Int.unsigned (s - 1)) in
-  serialize_tag_loop n (s * Int.repr  7 - Int.repr 7) tval
-                     ++[(tval >> Int.repr 2) & Int.repr 127]. 
-
+Definition serialize_length l := 
+  let s := required_size l in
+  let n := Z.to_nat (Int.unsigned s) in
+  (Int.repr 128 or s) :: serialize_length_loop ((s - 1) * Int.repr 8) n l.
+ 
 Definition ber_tlv_length_serialize len size : list int * int :=
    if (127 >=? Int.signed len)%Z then
     if eq_dec size 0 
     then ([], 1)
     else ([len], 1) 
-  else if (size <=u required_size len) 
-       then ([], required_size len + 1)
-       else ([],1).
+  else let r := required_size len in 
+       if (r <u size) 
+       then (serialize_length len, r + 1) 
+       else ([], r + 1).
 
