src/Lib/DWT/VSTber_tlv_tag_serialize.v
@@ -47,7 +47,6 @@ Definition ber_tlv_tag_serialize_spec' : ident * funspec :=
 
 Definition Gprog' := ltac:(with_library prog [ber_tlv_tag_serialize_spec']).
 
-Open Scope IntScope.
 
 Theorem ber_tlv_tag_serialize_correct' : 
   semax_body Vprog Gprog' (normalize_function f_ber_tlv_tag_serialize composites)
